powerpc/Conventions1.v
@@ -349,8 +349,9 @@ Proof.
   reflexivity.
 Qed.
 
-(** ** Normalization of function results *)
+(** ** Normalization of function results and parameters *)
 
 (** No normalization needed. *)
 
 Definition return_value_needs_normalization (t: rettype) := false.
+Definition parameter_needs_normalization (t: rettype) := false.
